\begin{problem}
    \normalfont
    Prove the following identities related to the cross product of vectors:
\begin{enumerate}
    \item 
    Prove the following:

\begin{align*}
(u\times v)\times w&=(u\cdot w)v-(v\cdot w)u\tag{1}\\[10pt]
\end{align*}


Converting from direct to indicial:

\begin{align*}
u&=u_{i}e_{i}\\[10pt]
v&=v_{j}e_{j}\\[10pt]
w&=w_{k}e_{k}
\end{align*}


\begin{align*}
(u\times v)\times w&=(u\cdot w)v-(v\cdot w)u\\[10pt]
&=(u_{i}e_{i}\times v_{j}e_{j})\times w_{k}e_{k}\\[10pt]
&=u_{i}v_{j}w_{k}(e_{i}\times e_{j})\times e_{k}\\[10pt]
&=u_{i}v_{j}w_{k}(\epsilon_{ijl}e_{l})\times e_{k}\\[10pt]
&=u_{i}v_{j}w_{k}\epsilon_{ijl}(e_{l}\times e_{k})\\[10pt]
&=u_{i}v_{j}w_{k}\epsilon_{ijl}\epsilon_{lkm}e_{m}\\[10pt]
&=u_{i}v_{j}w_{k}\epsilon_{ijl}\epsilon_{kml}e_{m}\\[10pt]
\end{align*}


Using the following identity:

$$
\epsilon_{ijl}\epsilon_{kml}=\delta_{ik}\delta_{jm}-\delta_{im}\delta_{jk}
$$


\begin{align*}
&=u_{i}v_{j}w_{k}(\delta_{ik}\delta_{jm}-\delta_{im}\delta_{jk})e_{m}\\[10pt]
&=v_{j}(u_{i}w_{k}\delta_{ik})\delta_{jm}e_{m}-u_{i}(v_{j}w_{k}\delta_{kj})\delta_{im}e_{m}\\[10pt]
&=v_{j}(u_{i}w_{i})e_{j}-u_{i}(v_{j}w_{j})e_{i}
\end{align*}

Converting back to direct notation:

\begin{align*}
v_{j}(u_{i}w_{i})e_{j}-u_{i}(v_{j}w_{j})e_{i}&=(u\times v)\times w\tag{2}
\end{align*}
Equation 1 and Equation 2 are equal. $\qed$
\vspace*{1cm}
\item
    Prove the following:


    \begin{align*}
    A\times(B\times C)&=B(A\cdot C)-C(A\cdot B)\\[10pt]
    \end{align*}
    
    
    Converting from direct to indicial:
    
    
    \begin{align*}
    A&=a_{i}e_{i}\\[10pt]
    B&=b_{j}e_{j}\\[10pt]
    C&=c_{k}e_{k}
    \end{align*}
    
    
    \begin{align*}
    A\times(B\times C)&=a_{i}e_{i}\times(b_{j}e_{j}\times c_{k}eK)\\[10pt]
    &=a_{i}b_{j}c_{k}e_{k}\times(e_{j}\times e_{k})\\[10pt]
    &=a_{i}b_{j}c_{k}e_{i}\times(\epsilon_{jkl}e_{l})\\[10pt]
    &=a_{i}b_{j}c_{k}\epsilon_{jkl}(e_{i}\times e_{l})\\[10pt]
    &=a_{i}b_{j}c_{k}\epsilon_{jkl}\epsilon_{ilm}e_{m}\\[10pt]
    &=a_{i}b_{j}c_{k}\epsilon_{jkl}\epsilon_{mil}e_{m}\\[10pt]
    \end{align*}

    \pagebreak
    Using the $\epsilon-\delta$ relation:
    

    \begin{align*}
    &=a_{i}b_{j}c_{k}(\delta_{jm}\delta_{ki}-\delta_{ji}\delta_{km})e_{m}\\[10pt]
    &=b_{j}(a_{i}c_{k}\delta_{ki})e_{m}-c_{k}(a_{i}b_{j}\delta_{ji})\delta_{km}e_{m}\\[10pt]
    &=b_{j}(A\cdot C)e_{j}-c_{k}(A\cdot B)e_{k}\\[10pt]
    &=B(A\cdot C)-C(A\cdot B)
    \end{align*}
    
    
    $\qed$
    
    
    \item     
Prove the following:
$$
\text{det}S=\frac{Su\cdot(Sv\times Sw)}{u\cdot(v\times w)}
$$

Converting from direct notation to indicial notation:

\begin{align*}
Su&=S_{ij}u_{j}e_{i}\\[10pt]
Sv&=S_{km}v_{m}e_{k}\\[10pt]
Sw&=S_{ol}w_{l}e_{o}
\end{align*}

\begin{align*}
u&=u_{j}e_{j}\\[10pt]
v&=v_{m}e_{m}\\[10pt]
w&=w_{l}e_{l}
\end{align*}


We can convert the numerator to the following:


\begin{align*}
Su\cdot(Sv\times Sw)&=(S_{ij}u_{j}e_{i})\cdot(S_{km}v_{m}e_{k}\times S_{ol}w_{l}e_{o})\\[10pt]
&=(S_{ij}u_{j}e_{i})\cdot(S_{km}v_{m}S_{ol}w_{l}(e_{k}\times e_{o}))\\[10pt]
&=(S_{ij}u_{j}e_{i})\cdot(S_{km}v_{m}S_{ol}w_{l}e_{p}\epsilon_{kop})\\[10pt]
&=\epsilon_{kop}S_{ij}u_{j}S_{km}v_{m}S_{ol}w_{l}(e_{l}\cdot e_{p})\\[10pt]
&=\epsilon_{kop}S_{ij}u_{j}S_{km}v_{m}S_{ol}w_{l}\delta_{ip}\\[10pt]
&=\epsilon_{koi}S_{ij}S_{km}S_{ol}u_{j}v_{m}w_{l}\tag{1}
\end{align*}
\pagebreak

Converting the denominator


\begin{align*}
u\cdot(v\times w)&=
(u_{j}e_{j})\cdot(v_{m}e_{m}\times w_{l}e_{l})\\[10pt]
&=(u_{j}e_{j})\cdot(v_{m}w_{l}(e_{m}\times e_{l}))\\[10pt]
&=(u_{j}e_{j})\cdot(v_{m}w_{l}e_{p}\epsilon_{mlp})\\[10pt]
&=\epsilon_{mlp}u_{j}v_{m}w_{l}\delta_{jp}\\[10pt]
&=\epsilon_{mlj}u_{j}v_{m}w_{l}\tag{2}
\end{align*}


Taking the ratio of Equation 1 and Equation 2:


\begin{align*}
\text{det}S &=\frac{\epsilon_{koi}S_{ij}S_{km}S_{ol}\cancel{ u_{j}v_{m}w_{l} }}{\epsilon_{mlj}\cancel{ u_{j}v_{m}w_{l} }}\\[10pt]
&=\frac{\epsilon_{koi}S_{ij}S_{km}S_{ol}}{\epsilon_{jml}}
\end{align*}


We know from the following identity:

$$
\epsilon_{jml} \ \text{det}S=\epsilon_{iko}S_{ij}S_{km}S_{ol}
$$

Dividing the above by $\epsilon_{jml}$:

$$
\text{det}S = \frac{\epsilon_{iko}S_{ij}S_{km}S_{ol}}{\epsilon_{jml}}
$$


Equation 3 and Equation 4 are equal. $\qed$
\end{enumerate}
\end{problem}
\pagebreak