\begin{problem} 
        \normalfont
        Prove the following identities:
    \begin{enumerate}

        \item $\mathbf{S}(\mathbf{u\otimes v})=(\mathbf{Su})\otimes \mathbf{v}$
        
        
\normalfont According to the definition of the tensor product, the left hand side can be multiplied by the following:

\begin{align*}
\mathbf{S}(\mathbf{u}\otimes \mathbf{v}) \mathbf{w}&=\mathbf{S(\mathbf{v}\cdot \mathbf{w})\mathbf{u}}\\[10pt]
&=(\mathbf{v}\cdot \mathbf{w})\mathbf{S}\mathbf{u}\tag{1}
\end{align*}

Multiplying by $\mathbf{w}$ on the right hand side:


\begin{align*}
(\mathbf{S}\mathbf{u}\otimes \mathbf{v})\mathbf{w}&=(\mathbf{v}\cdot \mathbf{w})(\mathbf{S}\mathbf{u})\tag{2}
\end{align*}


Equation 1 and Equation 2 are equal after being both multiplied by $\mathbf{w}$. \qed
\vspace*{1cm}
        \item $(\mathbf{u}\otimes \mathbf{v})\mathbf{S}=\mathbf{u}\otimes(\mathbf{S^T}\mathbf{v})$

        Taking the transpose of both sides then multiplying by $\mathbf{w}$ yields:
        
        
        \begin{align*}
        ((\mathbf{u}\otimes \mathbf{v})\mathbf{S})^T\mathbf{w}&=\mathbf{S}^T(\mathbf{v}\otimes \mathbf{u})\cdot \mathbf{w}\\[10pt]
        &=\mathbf{S}^T(\mathbf{u}\cdot \mathbf{w})\mathbf{v}
        \end{align*}
        
        
        Right hand side:
        
        
        \begin{align*}
        (\mathbf{u}\otimes (\mathbf{S}^T\mathbf{v}))^T&=((\mathbf{S}^T\mathbf{v})\otimes \mathbf{u})\mathbf{\mathbf{w}}=(\mathbf{u}\cdot \mathbf{w})\mathbf{S}^T\mathbf{v}\\[10pt]
        &=\mathbf{S}^T(\mathbf{u}\cdot \mathbf{w})\mathbf{v}
        \end{align*}
        
        
        The LHS and RHS are equal. \qed
        \pagebreak
        \item $(\mathbf{a}\otimes \mathbf{b})(\mathbf{c}\otimes \mathbf{d})=(\mathbf{b}\cdot \mathbf{c})\mathbf{a}\otimes \mathbf{d}$
        
        Using the identity below:

$$
\mathbf{S}(\mathbf{u\otimes v})=(\mathbf{Su})\otimes \mathbf{v}
$$


\begin{align*}
(\mathbf{a}\otimes \mathbf{b})(\mathbf{c}\otimes \mathbf{d})&=(\mathbf{b}\cdot \mathbf{c})\mathbf{a}\otimes \mathbf{d}\\[10pt]
\end{align*}

Multiplying both sides by $\mathbf{w}$:


\begin{align*}
(((\mathbf{b}\cdot \mathbf{c})\mathbf{a})\otimes \mathbf{d})\mathbf{w}&=(\mathbf{d}\cdot \mathbf{w})((\mathbf{b}\cdot \mathbf{c})\mathbf{a})
\end{align*}

Multiplying the RHS by $\mathbf{w}$:

$$
((\mathbf{b}\cdot \mathbf{c})\mathbf{a}\otimes \mathbf{d})\mathbf{w}=(\mathbf{d}\cdot \mathbf{w})((\mathbf{b}\cdot \mathbf{c})\mathbf{a})
$$

The LHS and RHS are equal. \qed
\vspace*{1cm}
        \item $\mathbf{R}\cdot(\mathbf{S}\mathbf{T})=(\mathbf{S}^T\mathbf{R})\cdot \mathbf{T}=(\mathbf{R}\mathbf{T}^T)\cdot \mathbf{S}$
        
        By the definition of the transpose:

$$
\mathbf{S}\mathbf{u}\cdot \mathbf{v}=\mathbf{u}\cdot \mathbf{S}^T\mathbf{v}
$$
Taking the transpose of each term:


\begin{align*}
(\mathbf{R}\cdot(\mathbf{S}\mathbf{T}))^T&=((\mathbf{S}^T\mathbf{R})\cdot \mathbf{T})^T=((\mathbf{R}\mathbf{T}^T)\cdot \mathbf{S})^T\\[10pt]
\implies \text{tr}(\mathbf{R}(\mathbf{S}\mathbf{T})^T)&=\text{tr}(\mathbf{S}^T\mathbf{R}\mathbf{T}^T)=\text{tr}((\mathbf{R}\mathbf{T}^T)\mathbf{S}^T)\\[10pt]\implies
\text{tr}(\mathbf{R}\mathbf{T^T}\mathbf{S^T})&=\text{tr}(\mathbf{R}\mathbf{T^T}\mathbf{S^T})=\text{tr}(\mathbf{R}\mathbf{T^T}\mathbf{S^T})\tag{1}
\end{align*}


Equation 1 are all equal. \qed
\pagebreak
        \item $\mathbf{S}\cdot(\mathbf{u}\otimes \mathbf{v})=\mathbf{u}\cdot \mathbf{S}\mathbf{v}$
        
        Taking the trace of the LHS:


\begin{align*}
\mathbf{S}\cdot(\mathbf{u}\otimes \mathbf{v})&=\text{tr}(\mathbf{S}(\mathbf{v}\otimes \mathbf{u}))\\[10pt]
&=\text{tr}((\mathbf{v}\otimes \mathbf{u})\mathbf{S})=\text{tr}(\mathbf{S\mathbf{v}}\otimes \mathbf{u})\\[10pt]
&=\mathbf{S}\mathbf{v}\cdot \mathbf{u}
\end{align*}


Dot products are commutative, so the LHS is equal to the S: 

$$
\mathbf{u}\cdot \mathbf{S}\mathbf{v}=\mathbf{S}\mathbf{v}\cdot \mathbf{u}
$$

\qed
\vspace*{1cm}
        \item $(\mathbf{a}\otimes \mathbf{b})\cdot(\mathbf{c}\otimes \mathbf{d})=(\mathbf{a}\cdot \mathbf{c})(\mathbf{b}\cdot \mathbf{d})$
        
        Taking the trace of the LHS:

        
        \begin{align*}
        (\mathbf{a}\otimes \mathbf{b})\cdot(\mathbf{c}\otimes \mathbf{d})&=\text{tr}((\mathbf{a}\otimes \mathbf{b})(\mathbf{d}\otimes \mathbf{c})\\[10pt]
        &=\text{tr}((\mathbf{b}\cdot \mathbf{d})\mathbf{a}\otimes \mathbf{c})\\[10pt]
        &=(\mathbf{b}\cdot \mathbf{d})\mathbf{a}\cdot \mathbf{c}=(\mathbf{b}\cdot \mathbf{d})(\mathbf{a}\cdot \mathbf{c})
        \end{align*}
        
        The LHS is equal to the RHS. \qed
    \end{enumerate}
\end{problem}
\pagebreak