\begin{problem}
    \noindent
    \normalfont
    \begin{enumerate}
    \item \begin{enumerate}
        \item First, we will compute the derivative of $R$ with respect to $\mathbf{X}_{i}$, as we will need these values for the main derivation of the deformation gradient:

        \begin{align}
        \mathbf{x}(\mathbf{X},t)=\frac{f(R,t)}{R}\mathbf{X}, \ R=\lvert \mathbf{X} \rvert  \\
        R = \sqrt{ \mathbf{X}_{1}^2+\mathbf{X}_{2}^2 +\mathbf{X}_{3}^2}  \\
        =\sqrt{ \mathbf{X}_{i}\mathbf{X}_{i} } \\
        \frac{ \partial R }{ \partial \mathbf{X}_{i} }=\frac{ \partial (\mathbf{X}_{i}\mathbf{X}_{i})^{1/2} }{ \partial \mathbf{X}_{k} }   \\
        =\frac{1}{2}(\mathbf{X}_{i}\mathbf{X}_{i})^{-\frac{1}{2}}\left( \frac{ \partial \mathbf{X}_{i} }{ \partial \mathbf{X}_{k} }  \mathbf{X}_{i}+\frac{ \partial \mathbf{X}_{i} }{ \partial \mathbf{X}_{K} }\mathbf{X}_{i} \right) \\
        =\frac{2\delta_{ik}\mathbf{X}_{i}}{2\sqrt{ \mathbf{X}_{i}\mathbf{X}_{i} }} \\
        =\frac{\mathbf{X}_{i}\mathbf{I}}{R}
        \end{align}
        
        We will compute the deformation gradient using the product rule:
        
        
        \begin{align}
        \mathbf{F}=\left( \frac{f(R,t)}{R}\mathbf{X}_{j} \right)_{i}=\frac{f(R,t)}{R}\underbrace{ \cancel{ \frac{ \partial \mathbf{X}_{j} }{ \partial \mathbf{X}_{i} } } }_{ \delta_{ij} } +\frac{ \partial  }{ \partial \mathbf{X}_{i} }\left( \frac{f(R,t)}{R} \right)\mathbf{X}_{j} \\
        =\frac{f(R,t)}{R}\mathbf{I}+\frac{ \partial  }{ \partial R } (f(R,t)R^{-1})\mathbf{X}_{j} \\
        =\frac{f(R,t)}{R}\mathbf{I}+\mathbf{X}_{j}\left( \frac{ \partial f(R,t) }{ \partial R }  \right)\frac{ \partial R }{ \partial \mathbf{X}_{j} } \frac{1}{R}+\left( \frac{ \partial R^{-1} }{ \partial R }  \right)\frac{ \partial R }{ \partial \mathbf{X}_{j} } f(R,t)\mathbf{X}_{j} \\
        =\frac{f(R,t)}{R}\mathbf{I}+\frac{ \partial f(R,t) }{ \partial R } \frac{(\mathbf{X}_{i})\mathbf{I}}{R} \frac{1}{R}\mathbf{X}_{j}+\left( -\frac{1}{R^2}\left( \frac{\mathbf{X}_{i}\mathbf{I}}{R} \right) \right)f(R,t)\mathbf{X}_{j} \\
        \end{align}
        \boxedeq{}{\mathbf{F}=\frac{f(R,t)}{R}\mathbf{I}+\frac{1}{R^2}\left( \frac{ \partial f }{ \partial R } -\frac{f}{R} \right)\mathbf{X}\otimes \mathbf{X}
        }
        \item The complete deformation gradient is given as follows:
    
        \begin{align}
        \mathbf{F}=\begin{bmatrix}
        \frac{f}{R}+\frac{1}{R^2}\left( \frac{ \partial f }{ \partial R } -\frac{f}{R} \right)\mathbf{X}_{1}^2 & \frac{1}{R^2}\left( \frac{ \partial f }{ \partial R } -\frac{f}{R} \right)\mathbf{X}_{1}\mathbf{X}_{2} & \frac{1}{R^2}\left( \frac{ \partial f }{ \partial R } -\frac{f}{R} \right)\mathbf{X_{1}\mathbf{X}_{3}} \\
        \frac{1}{R^2}\left( \frac{ \partial f }{ \partial R } -\frac{f}{R} \right)\mathbf{X_{1}\mathbf{X}_{3}}  &  \frac{f}{R}+\frac{1}{R^2}\left( \frac{ \partial f }{ \partial R } -\frac{f}{R} \right)\mathbf{X}_{2}^2 & \frac{1}{R^2}\left( \frac{ \partial f }{ \partial R } -\frac{f}{R} \right)\mathbf{X_{2}\mathbf{X}_{3}} \\
        \frac{1}{R^2}\left( \frac{ \partial f }{ \partial R } -\frac{f}{R} \right)\mathbf{X_{1}\mathbf{X}_{3}} & \frac{1}{R^2}\left( \frac{ \partial f }{ \partial R } -\frac{f}{R} \right)\mathbf{X_{2}\mathbf{X}_{3}} & \frac{f}{R}+\frac{1}{R^2}\left( \frac{ \partial f }{ \partial R } -\frac{f}{R} \right)\mathbf{\mathbf{X}}_{3}^2
        \end{bmatrix}
        \end{align}
    
        
        Computing the determinant:
        
    
        \begin{align}
        \det(\mathbf{F})=\frac{1}{R^5}\left[ R^2\mathbf{F}^3+Rf^2\frac{ \partial \mathbf{F} }{ \partial R } (\mathbf{X}_{1}^2+\mathbf{X}_{2}^2+\mathbf{X}_{3}^2)-\mathbf{F}(\mathbf{X}_{1}^2+\mathbf{X}_{2}^2+\mathbf{X}_{3}^2) \right] \\
        \end{align}
        
        
        Substituting $R^2=\mathbf{X}_{1}^2+\mathbf{X}_{2}^2+\mathbf{X}_{3}^2$:
        
        
        \begin{align}
        \frac{1}{R^5}\left[ R^2\mathbf{F}^3+R^3f^2\frac{ \partial \mathbf{F} }{ \partial R } R^2\mathbf{F}^3 \right] \\
        =\frac{1}{R^5}R^3\mathbf{F}^2\frac{ \partial F }{ \partial R } =\frac{\mathbf{F}^2}{R^2}\frac{ \partial \mathbf{F} }{ \partial R }  \\
        \end{align}
        \boxedeq{}{\det(\mathbf{F})=\left( \frac{f}{R} \right)^2\frac{ \partial f }{ \partial R }}
    
    \end{enumerate}
    \item To compute the material velocity and acceleration fields, we simply take the time derivatives:
    
    \begin{align}
    \mathbf{x}(\mathbf{X},t)=\frac{f(R,t)}{R}\mathbf{X} \\
    \end{align}
    \boxedeq{}{\mathbf{v}=\frac{\mathbf{X}}{R}\dot{f} \\
    \mathbf{a}=\frac{\mathbf{X}}{R}\ddot{f}}
    
    
    To compute the spatial velocity and acceleration fields, we find and substitute the inverse map $\mathbf{X}=\frac{\mathbf{x}R}{f}$ into the material velocity field, and the spatial acceleration field is found by applying the formula below:
    
    
    \begin{align}
    \mathbf{a}_{s}=\mathbf{v}_{s}+\text{grad}(\mathbf{v}_{s})\mathbf{v_{s}}
    \end{align}
    
    Computing the spatial fields:
    
    \begin{align}
    \mathbf{v}_{s}=\left( \frac{\mathbf{x}R}{fR} \right)\dot{f}=\left( \frac{\mathbf{x}}{f} \right)\dot{f} \\
    \mathbf{a}_{s}=\frac{\mathbf{x}\ddot{f}}{f}+\mathbf{x}\dot{f}(-f^{-2})+\text{grad}(\mathbf{v}_{s})\mathbf{v}_{s} \\
    \end{align}
    \boxedeq{}{\mathbf{v}_{s}=\left( \frac{\mathbf{x}}{f} \right)\dot{f}\\\mathbf{a}_{s}=\frac{\mathbf{x}\ddot{f}}{f}-\frac{\mathbf{x}\dot{f}}{f^2}+\frac{\mathbf{x}\dot{f}^2}{f^2}
    }
    \item Performing separation of variables:
    
    \begin{align}
    \det(\mathbf{F})=\frac{f^2}{R^2}\frac{ \partial \mathbf{F} }{ \partial R } =1\implies \mathbf{F}^2\partial \mathbf{F}=R^2\partial \mathbf{F} \\
    \frac{1}{3}\mathbf{F}^3=\frac{1}{3}R^3+p(t)+C \\
    \mathbf{x}(\mathbf{X},t)=\frac{f(R,t)}{R}\mathbf{X}, \mathbf{X}=a_{0}
    \end{align}
    
    
    Using the initial conditions such that $\mathbf{X}=a_{0}, R=a_{0}$, this implies that $x(a_{0},t)=f(a_{0}, t)$ and $\mathbf{x}(a_{0}, t)=\mathbf{F}(a_{0},t)=a(t)$:
    
    
    \begin{align}
    \mathbf{F}^3=R^3+p(t)+C \\
    =F(a_{0}, t)^3=a(t)^3=a_{0}^3+p(t)+C, p(t)=a(t)^3, C = -a_{0}^3 \\
    f(R,t)^3=R^3+a(t)^3-a_{0}^3 \\
    \end{align}
    \boxedeq{}{f(R,t)=(R^3+a(t)^3-a_{0}^3)^{\frac{1}{3}}}
    \end{enumerate}
    
\end{problem}
\pagebreak