\begin{problem}
    \noindent
    \normalfont

    
\begin{align}
\lambda_{3}\to n=v_{3} \\
\lvert N \rvert = \lvert T\mathbf{n}\cdot \mathbf{n} \rvert \leq \lvert T\mathbf{v}_{3}\cdot v_{3} \rvert \\
= \lvert \lambda \mathbf{v}_{3}\cdot \mathbf{v}_{3} \rvert \\
\implies \parallel T \mathbf{n} \cdot \mathbf{n}\parallel \leq \lvert \lambda_{3} \rvert 
\end{align}


\begin{align}
\lvert T \mathbf{n}\cdot \mathbf{n} \rvert =  \\
\lvert T(k_{1}\mathbf{v}_{1}+k_{2}\mathbf{v}_{2}+k_{3}\mathbf{v}_{3})\cdot(k_{1}\mathbf{v}_{1}+k_{2}\mathbf{v}_{2}+k_{3}\mathbf{v}_{3})\rvert   \\
= \lvert k_{1}T\mathbf{v}_{1}+k_{2}T\mathbf{v}_{2}+k_{3}Tv_{3} \cdot k_{1}T\mathbf{v}_{1}+k_{2}T\mathbf{v}_{2}+k_{3}Tv_{3}\rvert  \\
= \lvert \lambda k_{1}\mathbf{v_{1}} + \lambda_{2}k_{2}\mathbf{v_{2}}+\lambda_{3}k_{3}\mathbf{v_{3}} \cdot \lambda_{1}k_{1}\mathbf{v_{1}} + \lambda_{2}k_{2}\mathbf{v_{2}}+\lambda_{3}k_{3}\mathbf{v_{3}}\rvert \\
= \lvert \lambda_{1}k_{1}^2+\lambda_{2}k_{2}^2+\lambda_{3}k_{3}^2 \rvert 
\end{align}

\begin{align}
\lambda_{1}\cos^2\theta_{1}+\lambda_{2}\cos^2\theta_{2}+\lambda_{3}\cos^2\theta_{3} \leq \lvert \lambda_{3}|(\cos^2\theta_{1}+\cos^2\theta_{2}+\cos^2\theta_{3}) \leq \lvert \lambda_{3} \rvert 
\end{align}
\end{problem}
